\begin{answer}
	$$
	\begin{aligned}
		\theta_{\text{MAP}} & = \arg\max_{\theta} p(y\mid x,\theta)\exp(-(bI)^{-1}|\theta|)\\
		& = \arg\max_{\theta} \left(\sum_{i=1}^m \ln p(y^{(i)} | x^{(i)}, \theta) -\frac{1}{b}|\theta|\right)\\
		& = \arg\min_{\theta} \left[(y - X\theta)^T(y - X\theta) + \frac{1}{b}|\theta|\right]\\
		& = \arg\min_{\theta} \left(\|X\theta-y\|_2^2 + \frac{1}{b}\|\theta\|_1\right)
	\end{aligned}
	$$
	
	Hence,
	
	$$
	J(\theta) = \|X\theta-y\|_2^2 + \lambda\|\theta\|_1\\
	$$
	
	$$
	\lambda = \frac{1}{b}
	$$
\end{answer}
