\begin{answer}
	\\
	For any $x$ lies in the decision boundary, we have $p(x|y=0)=p(x|y=1)$, which can be written as
	
	$$
	(x - \mu_0)^T \Sigma^{-1} (x - \mu_0)=(x - \mu_1)^T \Sigma^{-1} (x - \mu_1)
	$$.
	
	Therefore,
	
	\begin{align*}
		\mathrm{LHS} &= x^T \sigma^{-1} x - x^T \sigma^{-1} \mu_0 - \mu_0^T \sigma^{-1} x + \mu_0^T \sigma^{-1} \mu_0\\
		\mathrm{RHS} &= x^T \sigma^{-1} x - x^T \sigma^{-1} \mu_1 - \mu_1^T \sigma^{-1} x + \mu_1^T \sigma^{-1} \mu_1
	\end{align*}
	
	Since $\Sigma$ is symmetric, so is $\Sigma^{-1}$, and then $x^T \sigma^{-1} \mu_0 = \mu_0^T \sigma^{-1} x$ (the same for $\mathrm{RHS}$).
	
	The equation can be writen as
	
	$$
	\mu_0^T \Sigma^{-1} \mu_0 - \mu_1^T \Sigma^{-1} \mu_1 = 2x^T \Sigma^{-1} (\mu_0 - \mu_1)
	$$
	
	Take transposes for both sides:
	
	$$
	\left(2\Sigma^{-1} (\mu_0 - \mu_1)^T\right) x = \mu_0^T \Sigma^{-1} \mu_0 - \mu_1^T \Sigma^{-1} \mu_1
	$$
	
	where $2\Sigma^{-1} (\mu_0 - \mu_1)^T$ is an $1 \times n$ matrix and $\mu_0^T \Sigma^{-1} \mu_0 - \mu_1^T \Sigma^{-1} \mu_1$ is a scalar. This implies that all possible $x$'s make up a hyperplane in $R^n$, so the decision boundary is linear.
	
	\begin{align*}
		& p(y = 1|x; \phi, \mu_0, \mu_1, \Sigma)\\
		= & \frac{p(x|y = 1; \phi, \mu_0, \mu_1, \Sigma)p(y = 1; \phi)}{p(x|y = 0; \phi, \mu_0, \mu_1, \Sigma)p(y = 0; \phi) + p(x|y = 1; \phi, \mu_0, \mu_1, \Sigma)p(y = 1; \phi)}\\
		= & \frac{\exp\left(-\frac{1}{2}(x-\mu_1)^T \Sigma^{-1} (x-\mu_1) \right) \phi}{\exp\left(-\frac{1}{2}(x-\mu_{0})^T \Sigma^{-1} (x-\mu_{0})\right) (1 - \phi) + \exp\left(-\frac{1}{2}(x-\mu_1)^T \Sigma^{-1} (x-\mu_1) \right) \phi}\\
		= & \frac{1}{1 + (\phi^{-1} - 1) \exp\left(\frac{1}{2}\left[(x-\mu_1)^T \Sigma^{-1} (x-\mu_1) - (x-\mu_0)^T \Sigma^{-1} (x-\mu_0)  \right]\right)}\\
		= & \frac{1}{1 + \exp\left(-2 (\mu_1 - \mu_0)^T \Sigma^{-1} x - (\mu_0^T \Sigma^{-1} \mu_0 - \mu_1^T \Sigma^{-1} \mu_1 - \ln (\phi^{-1} - 1))\right)}\\
	\end{align*}
	
	Let $\theta = 2 (\mu_1 - \mu_0) \Sigma^{-1}$ and $\theta_0 = \mu_0^T \Sigma^{-1} \mu_0 - \mu_1^T \Sigma^{-1} \mu_1 - \ln (\phi^{-1} - 1)$, and then $p(y = 1|x; \phi, \mu_0, \mu_1, \Sigma) = \frac{1}{1 + \exp(-(\theta^T x + \theta_0))}$
\end{answer}