\begin{answer}
	\\
	Given $p(t^{(i)} = 1 | y^{(i)} = 1) = 1$, we have
	
	$$
	\begin{aligned}
		p(y^{(i)} = 1, t^{(i)} = 1 | x^{(i)}) & = p(y^{(i)} = 1| x^{(i)}) p(t^{(i)} = 1 | y^{(i)} = 1, x^{(i)})\\
		& = p(y^{(i)} = 1| x^{(i)})
	\end{aligned}
	$$
	
	Hence,
	
	$$
	\begin{aligned}
		p(y^{(i)} = 1| x^{(i)}) & = p(y^{(i)} = 1, t^{(i)} = 1 | x^{(i)})\\
		& = p(t^{(i)} = 1 | x^{(i)}) p(y^{(i)} = 1 | t^{(i)} = 1, x^{(i)})\\
		& = p(t^{(i)} = 1 | x^{(i)}) p(y^{(i)} = 1 | t^{(i)} = 1)
	\end{aligned}
	$$
	
	It turns out that $p(y^{(i)} = 1 | t^{(i)} = 1)$ is a constant since the dataset is distributed to a fixed distribution. So let $\alpha = p(y^{(i)} = 1 | t^{(i)} = 1)$, we obtain $p(t^{(i)} = 1 | x^{(i)}) = p(y^{(i)} = 1 | x^{(i)}) / \alpha$.
\end{answer}
